Some tests now run
make build-ExtractionTest
make build-Examples.Intro
make build-Examples.Guess
make build-Examples.Autograder

state/Test_Examples.Intro.ml
@@ -1,1 +1,9 @@
 open Examples_Intro
+
+let _ =
+  let r = whole_triv () in
+  print_string ("triv returned " ^ string_of_int (Z.to_int r) ^ "\n")
+
+let _ =
+  let r = whole_adv () in
+  print_string ("adv returned " ^ string_of_int (Z.to_int r) ^ "\n")
