state/Examples.Intro.fst
@@ -40,7 +40,8 @@ let sit : src_interface1 = {
   psi = fun _ _ _ -> True
 }
 
-#push-options "--z3rlimit 10000"
+#push-options "--z3rlimit 50" (* very flaky for some reason. *)
+#restart-solver
 let prog (lib : lib_type concrete_spec) : SST int (requires fun h0 -> True) (ensures fun h0 _ h1 -> True) =
   let secret : ref int = sst_alloc 42 in
   let r : ref (ref int) = sst_alloc_shared #(SRef SNat) (sst_alloc_shared 0) in
@@ -50,7 +51,8 @@ let prog (lib : lib_type concrete_spec) : SST int (requires fun h0 -> True) (ens
   let v : ref int = sst_alloc_shared 1 in
   sst_write r v;
   cb ();
-  assert (!secret == 42);
+  let v = !secret in
+  assert (v == 42);
   0
 #pop-options
 
